project/inductive/basic/inductive_graph_basic_theory.v
@@ -1,0 +1,167 @@
+Require Import String.
+Require Import Coq.Arith.Arith.
+Open Scope string_scope.
+
+Require Import List.
+Require Import Bool.
+Import ListNotations.
+
+Require Import MyProject.project.inductive.basic.inductive_graph_basic.
+Require Import MyProject.project.relational_graph.
+
+Require Import Coq.Sets.Ensembles.
+
+
+(* Defining Conversion from basic Inductive Graph to Relational Graph *)
+
+
+(* Adds a node and its in- and out- going edges (= its IG context) to an RG.
+    Assumes that the neighboring nodes exist *)
+Definition _extendByContext (node : Node) (froms tos : NatSet.t) (rg : RG nat) : RG nat.
+Proof.
+    refine {|
+        gr_nodes := fun (n : nat) => n = node \/ NatSet.In n froms \/ NatSet.In n tos \/ rg.(gr_nodes) n;
+
+        gr_edges := fun (n0 n1 : nat) =>
+                                (NatSet.In n0 froms /\ n1 = node)
+                                \/ (n0 = node /\ NatSet.In n1 tos)
+                                \/ rg.(gr_edges) n0 n1
+                                ;
+                     
+        gr_valid := _
+    |}.
+    unfold valid_cond. pose proof rg.(gr_valid). firstorder.
+Defined.
+
+
+Definition _accTo_RG (node : Node) (rgIg : RG nat * IG) : RG nat * IG :=
+    match rgIg with | (rg, ig) =>
+        match matsh node ig with
+        | (Some (froms, tos), rest) => (_extendByContext node froms tos rg, rest)
+        | (None, sameIg)            => (rg, sameIg)
+        end
+    end
+.
+
+Definition IG_basic_to_RG (ig : IG) : RG nat :=
+    match fold_right _accTo_RG (RG_empty, ig) (labNodes ig) with
+    | (rg, acc) => rg
+    end
+.
+
+
+(* Coercion IG_basic_to_RG : IG >-> RG. *)
+
+Definition equiv_IG (ig1 ig2 : IG) : Prop :=
+    equiv_G (IG_basic_to_RG ig1) (IG_basic_to_RG ig2)
+.
+
+Notation "g1 I== g2" := (equiv_IG g1 g2) (at level 80).
+
+
+(* Section to make rewrite work with equiv_IG *)
+
+(* Source for rewrite: https://stackoverflow.com/questions/56099646/use-rewrite-tactic-with-my-own-operator-in-coq *)
+Require Import Setoid Morphisms.
+
+(* This proof is based on === being an equivalence relation *)
+Instance IG_Equivalence_eq : Equivalence equiv_IG.
+Proof.
+    pose proof (@RG_Equivalence_eq nat). destruct H. split.
+    - unfold Reflexive. intros. unfold Reflexive in Equivalence_Reflexive. apply Equivalence_Reflexive.
+    - unfold Symmetric. intros. unfold Symmetric in Equivalence_Symmetric. apply Equivalence_Symmetric. apply H.
+    - unfold Transitive. intros. unfold Transitive in Equivalence_Transitive. apply (Equivalence_Transitive _ (IG_basic_to_RG y) _).
+        + apply H.
+        + apply H0.
+Qed. 
+
+
+Example basic_equivalence_test : (mkGraph [1; 2] []) I== (mkGraph [2; 1] []).
+Proof.
+    unfold equiv_IG. unfold equiv_G. firstorder.
+Qed.
+
+Example basic_equivalence_test' : (mkGraph [1; 2; 3] [(1, 2); (2, 3)]) I== (mkGraph [2; 1; 3] [(2, 3); (1, 2)]).
+Proof.
+    unfold equiv_IG. unfold equiv_G. firstorder.
+Qed.
+
+
+
+(* Now start defining the basic IG functions in terms of an RG *)
+  (* {-# MINIMAL empty, isEmpty, match, mkGraph, labNodes #-} *)
+
+
+(* Start defining functionality: *)
+Definition RG_empty : RG nat :=
+    RG_empty.
+
+
+Definition RG_isEmpty (rg : RG nat) : Prop :=
+  RG_isEmpty rg.
+
+
+
+(* Helper for matsh *)
+Definition _eliminate (node : Node) (rg : RG nat) : RG nat.
+Proof.
+  refine {|
+      gr_nodes :=  Subtract nat (rg.(gr_nodes)) node;
+      gr_edges := fun (n0 n1 : nat) => n0 <> node /\ n1 <> node /\  rg.(gr_edges) n0 n1;
+      gr_valid := _
+  |}.
+  unfold valid_cond. pose proof rg.(gr_valid). firstorder.
+  - unfold not. intros. inversion H2. congruence.
+  - unfold not. intros. inversion H2. congruence.
+Defined.
+
+Definition _getFromsAndTos (node : Node) (rg : RG nat) : Prop * (Ensemble nat * Ensemble nat) :=
+  (rg.(gr_nodes) node, ((fun (from : nat) => rg.(gr_edges) from node), (fun (to : nat) => rg.(gr_edges) node to)))
+.
+
+
+(* (Ensemble nat * Ensemble nat) is not a relation, it is two _independent_ sets of from- and to- neighbors *)
+Definition RG_matsh (node : Node) (rg : RG nat) : (Prop * (Ensemble nat * Ensemble nat)) * RG nat :=
+  (_getFromsAndTos node rg, _eliminate node rg)
+.
+
+
+
+Definition _add (node : Node) (fromsTos : (NatSet.t * NatSet.t)) (rg : RG nat) : RG nat :=
+  match fromsTos with | (froms, tos) =>
+    _extendByContext node froms tos rg
+  end
+.
+
+
+Definition _insNode (node : Node) (rg : RG nat) : RG nat :=
+  _add node (NatSet.empty, NatSet.empty) rg.
+  
+
+Definition _insNodes (nodes : list Node) (rg : RG nat) : RG nat :=
+  fold_right _insNode rg nodes.
+
+
+(* If one of the nodes of the edge does not exist, nothing happens *)
+Definition _insEdge (edge : (Node * Node)) (rg : RG nat) : RG nat.
+Proof.
+  destruct edge as [node0 node1].
+    refine {|
+      gr_nodes := rg.(gr_nodes);
+      gr_edges := fun (n0 n1 : nat) => (n0 = node0 /\ n1 = node1 /\ rg.(gr_nodes) node0 /\ rg.(gr_nodes) node1) \/  rg.(gr_edges) n0 n1;
+      gr_valid := _
+  |}.
+  unfold valid_cond. pose proof rg.(gr_valid). firstorder.
+  - congruence.
+  - congruence.
+Qed.
+
+
+Definition _insEdges (edges : list (Node * Node)) (rg : RG nat) : RG nat :=
+  fold_right _insEdge rg edges.
+
+Definition RG_mkGraph (nodes : list Node) (edges : list (Node * Node)) : RG nat :=
+  _insEdges edges (_insNodes nodes RG_empty).
+ 
+Definition RG_labNodes (rg : RG nat) : Ensemble Node :=
+  rg.(gr_nodes).
